isabelle/CVM_Subsample/CVM_Original_Algorithm.thy
@@ -1,0 +1,259 @@
+theory CVM_Original_Algorithm
+  imports CVM_Abstract_Algorithm
+begin
+
+context
+  fixes f :: real
+  fixes thresh :: nat
+  assumes f_range: \<open>f \<in> {1/2..exp(-1/12)}\<close>
+  assumes thresh_gt_0: \<open>thresh > 0\<close>
+begin
+
+definition initial_state :: \<open>'a state\<close> where
+  \<open>initial_state \<equiv> \<lparr>state_k = 0, state_chi = {}\<rparr>\<close>
+
+definition step_1 :: \<open>'a \<Rightarrow> 'a state \<Rightarrow> 'a state spmf\<close> where
+  \<open>step_1 x \<sigma> = 
+    do {
+      let k = state_k \<sigma>;
+      let chi = state_chi \<sigma>; 
+
+      insert_x_into_chi \<leftarrow> bernoulli_pmf (f ^ k);
+
+      let chi = (chi |>
+        if insert_x_into_chi
+        then insert x
+        else Set.remove x);
+
+      return_spmf (\<sigma>\<lparr>state_chi := chi\<rparr>)
+    }\<close>
+
+definition subsample :: \<open>'a set \<Rightarrow> 'a set spmf\<close> where
+  \<open>subsample U =
+    do {
+      keep_in_chi \<leftarrow> prod_pmf U (\<lambda>_. bernoulli_pmf f);
+      return_spmf (Set.filter keep_in_chi U)
+    }\<close>
+ 
+definition step_2 :: \<open>'a state \<Rightarrow> 'a state spmf\<close> where
+  \<open>step_2 \<sigma> = 
+    do {
+      let k = state_k \<sigma>;
+      let chi = state_chi \<sigma>;
+  
+      if card chi = thresh
+      then (chi
+        |> subsample
+        |> map_spmf (\<lambda> chi. \<lparr>state_k = k + 1, state_chi = chi\<rparr>))
+      else return_spmf \<sigma>
+    }\<close>
+
+definition step_3 :: \<open>'a state \<Rightarrow> 'a state spmf\<close> where
+  \<open>step_3 \<sigma> = 
+    do {
+      let chi = state_chi \<sigma>;
+  
+      if card chi = thresh
+      then fail_spmf
+      else return_spmf \<sigma>
+    }\<close>
+
+definition run_steps :: \<open>'a list \<Rightarrow> 'a state spmf\<close> where
+  \<open>run_steps xs \<equiv> foldM_spmf (\<lambda>x \<sigma>. step_1 x \<sigma> \<bind> step_2 \<bind> step_3) xs initial_state\<close>
+
+definition estimate :: \<open>'a state \<Rightarrow> real\<close> where
+  \<open>estimate \<sigma> = card (state_chi \<sigma>) / f ^ state_k \<sigma>\<close>
+
+lemma ord_spmf_remove_step3:
+  \<open>ord_spmf (=) (step_1 x \<sigma> \<bind> step_2 \<bind> step_3) (step_1 x \<sigma> \<bind> step_2)\<close>
+proof -
+  have \<open>ord_spmf (=) (local.step_2 x \<bind> local.step_3) (local.step_2 x)\<close> for x :: \<open>'a state\<close>
+  proof -
+    have \<open>ord_spmf (=) (local.step_2 x \<bind> local.step_3) (local.step_2 x \<bind> return_spmf)\<close>
+      by (intro bind_spmf_mono') (simp_all add:step_3_def)
+    thus ?thesis by simp
+  qed
+  thus ?thesis unfolding bind_spmf_assoc by (intro bind_spmf_mono') simp_all
+qed
+
+lemma ord_spmf_run_steps: 
+  \<open>ord_spmf (=) (run_steps xs) (foldM_spmf (\<lambda>x \<sigma>. step_1 x \<sigma> \<bind> step_2) xs initial_state)\<close>
+  unfolding run_steps_def
+proof (induction xs rule:rev_induct)
+  case Nil
+  then show ?case by simp 
+next
+  case (snoc x xs)
+  show ?case
+    unfolding run_steps_def foldM_spmf_snoc
+    by (intro ord_spmf_remove_step3 bind_spmf_mono' snoc)
+qed
+
+lemma f_range_simple: \<open>f \<in> {1/2..<1}\<close>
+proof -
+  have \<open>exp (- 1 / 12) < (1::real)\<close> by (approximation 5)
+  from dual_order.strict_trans2[OF this]
+  show ?thesis using f_range by auto
+qed
+
+theorem correctness:
+  fixes xs :: \<open>'a list\<close>
+  assumes \<open>\<epsilon> \<in> {0<..<1}\<close> \<open>\<delta> \<in> {0<..<1}\<close>
+  assumes \<open>real thresh \<ge> 12 / \<epsilon> ^ 2 * ln (6 * real (length xs) / \<delta>)\<close>
+  defines \<open>R \<equiv> real (card (set xs))\<close>
+  shows \<open>measure (run_steps xs) {\<omega>. fails_or_satisfies (\<lambda>x. \<bar>estimate x - R\<bar> > \<epsilon> * R) \<omega>} \<le> \<delta>\<close>
+    (is \<open>?L \<le> ?R\<close>)
+proof -
+  define abs_subsample where 
+    \<open>abs_subsample U = map_pmf (\<lambda>\<omega>. Set.filter \<omega> U) (prod_pmf U (\<lambda>_. bernoulli_pmf f))\<close>
+    for U :: \<open>'a set\<close>
+
+  interpret abs:cvm_algo_abstract thresh f abs_subsample
+    rewrites \<open>abs.estimate = estimate\<close>
+  proof -
+    show abs:\<open>cvm_algo_abstract thresh f abs_subsample\<close>
+    proof (unfold_locales, goal_cases)
+      case 1 thus ?case by (rule thresh_gt_0)
+    next
+      case 2 thus ?case using f_range_simple by auto
+    next
+      case (3 U x)
+      then show ?case unfolding abs_subsample_def by auto
+    next
+      case (4 g U S)
+      hence fin_U: \<open>finite U\<close> using thresh_gt_0 card_gt_0_iff by metis
+      note conv = Pi_pmf_subset[OF this 4(1)]
+
+      have \<open>(\<integral>\<omega>. (\<Prod>s\<in>S. g (s \<in> \<omega>)) \<partial>abs_subsample U) = 
+        (\<integral>\<omega>. (\<Prod>s\<in>S. g (s \<in> U \<and> \<omega> s)) \<partial>prod_pmf U (\<lambda>_. bernoulli_pmf f))\<close> 
+        unfolding abs_subsample_def by (simp cong:prod.cong)
+      also have \<open>\<dots> = (\<integral>\<omega>. (\<Prod>s\<in>S. g (s \<in> U \<and> \<omega> s)) \<partial>prod_pmf S (\<lambda>_. bernoulli_pmf f))\<close>
+        unfolding conv by simp
+      also have \<open>\<dots> = (\<Prod>s\<in>S. (\<integral>\<omega>. g (s \<in> U \<and> \<omega>) \<partial>bernoulli_pmf f))\<close> 
+        using fin_U finite_subset[OF 4(1)] 
+        by (intro expectation_prod_Pi_pmf integrable_measure_pmf_finite) auto
+      also have \<open>\<dots> = (\<Prod>s\<in>S. (\<integral>\<omega>. g \<omega> \<partial>bernoulli_pmf f))\<close> 
+        using 4(1) by (intro prod.cong refl) auto
+      finally show ?case by simp
+    qed
+    show \<open>cvm_algo_abstract.estimate f = (estimate :: 'a state \<Rightarrow> real)\<close> 
+      unfolding cvm_algo_abstract.estimate_def[OF abs] estimate_def by simp
+  qed
+
+  have a: \<open>step_1 \<sigma> x = spmf_of_pmf (abs.step_1 \<sigma> x)\<close> for \<sigma> x
+    unfolding step_1_def abs.step_1_def spmf_of_pmf_def by (simp add:map_bind_pmf)
+
+  have b: \<open>step_2 \<sigma> = map_pmf Some (abs.step_2 \<sigma>)\<close> for \<sigma> 
+    unfolding step_2_def abs.step_2_def subsample_def abs_subsample_def 
+    by (simp add:map_bind_pmf Let_def map_pmf_def[symmetric] map_pmf_comp)
+
+  have c: \<open>abs.initial_state = initial_state\<close> 
+    unfolding initial_state_def abs.initial_state_def by simp
+
+  have d: \<open>subsample U = spmf_of_pmf (abs_subsample U)\<close> for U
+    unfolding subsample_def abs_subsample_def map_pmf_def[symmetric] 
+    by (simp add:spmf_of_pmf_def map_pmf_comp)
+
+  define \<alpha> :: real where \<open>\<alpha> = f ^ thresh\<close>
+
+  have \<alpha>_range: \<open>\<alpha> \<in> {0..1}\<close> 
+    using f_range_simple unfolding \<alpha>_def by (auto intro:power_le_one)
+  hence [simp]: \<open>\<bar>\<alpha>\<bar> \<le> 1\<close> by auto
+
+  have \<open>(\<integral>x. (if card x = thresh then 1 else 0) \<partial>abs_subsample U) \<le> \<alpha>\<close> (is \<open>?L1 \<le> _\<close>)
+    if that': \<open>card U = thresh\<close> for U
+  proof -
+    have fin_U: \<open>finite U\<close> using thresh_gt_0 that card_gt_0_iff by metis
+
+    have \<open>(\<Prod>s\<in>U. of_bool (s \<in> x)::real) = of_bool(card x = thresh)\<close>
+      if \<open>x \<in> set_pmf (abs_subsample U)\<close> for x
+    proof -
+      have x_ran: \<open>x \<subseteq> U\<close> using that unfolding abs_subsample_def by auto
+
+      have \<open>(\<Prod>s\<in>U. of_bool (s \<in> x)::real) = of_bool(x = U)\<close>
+        using fin_U x_ran by (induction U rule:finite_induct) auto 
+      also have \<open>\<dots> = of_bool (card x = card U)\<close>
+        using x_ran fin_U card_subset_eq by (intro arg_cong[where f=\<open>of_bool\<close>]) blast
+      also have \<open>\<dots> = of_bool (card x = thresh)\<close> using that' by simp
+      finally show ?thesis by auto 
+    qed
+    hence \<open>?L1 = (\<integral>x. (\<Prod>s \<in> U. of_bool(s \<in> x)) \<partial>abs_subsample U)\<close>
+      by (intro integral_cong_AE AE_pmfI) simp_all
+    also have \<open>\<dots> \<le> (\<Prod>s \<in> U. (\<integral>x. of_bool x \<partial>bernoulli_pmf f))\<close>
+      by (intro abs.subsample_inequality that) auto
+    also have \<open>\<dots> = f ^ card U\<close> using f_range_simple by simp
+    also have \<open>\<dots> = \<alpha>\<close> unfolding \<alpha>_def that by simp
+    finally show ?thesis by simp
+  qed
+  hence e: \<open>pmf (step_2 \<sigma> \<bind> step_3) None \<le> \<alpha>\<close> for \<sigma> :: \<open>'a state\<close> 
+    using \<alpha>_range unfolding step_2_def step_3_def d 
+    by (simp add:Let_def bind_map_pmf comp_def pmf_bind if_distrib if_distribR cong:if_cong)
+
+  have \<open>pmf (step_1 x \<sigma> \<bind> step_2 \<bind> step_3) None \<le> \<alpha>\<close> for \<sigma> and x :: 'a
+  proof-
+    have \<open>pmf (step_1 x \<sigma> \<bind> step_2 \<bind> step_3) None \<le> 0 + (\<integral>_. \<alpha> \<partial> measure_spmf (step_1 x \<sigma>))\<close> 
+      unfolding bind_spmf_assoc pmf_bind_spmf_None[where p=\<open>step_1 x \<sigma>\<close>]
+      by (intro add_mono integral_mono_AE measure_spmf.integrable_const_bound[where B=\<open>1\<close>] 
+          iffD2[OF AE_measure_spmf_iff] ballI e)
+         (simp_all add:pmf_le_1 step_1_def map_pmf_def[symmetric] pmf_map vimage_def)
+    also have \<open>\<dots> \<le> \<alpha>\<close> using \<alpha>_range by (simp add: mult_left_le_one_le weight_spmf_le_1) 
+    finally show ?thesis by simp
+  qed
+  hence \<open>prob_fail (run_steps xs) \<le> length xs * \<alpha>\<close>
+    unfolding run_steps_def by (intro prob_fail_foldM_spmf_le[where P=\<open>\<lambda>_. True\<close>]) auto
+  also have \<open>\<dots> \<le> \<delta> / 2\<close>
+  proof (cases \<open>xs = []\<close>)
+    case True
+    thus ?thesis using assms(2) by auto
+  next 
+    case False
+    have \<open>\<delta> \<le> 6 * 1\<close> using assms(2) by simp
+    also have \<open>\<dots> \<le> 6 * real (length xs)\<close>
+      using False by (intro mult_mono order.refl) (cases xs, auto) 
+    finally have [simp]: \<open> \<delta> \<le> 6 * real (length xs)\<close> by simp
+    have \<open>2 * real (length xs) * f ^ thresh \<le> 2 * real (length xs) * exp (-1/12)^thresh\<close>
+      using f_range by (intro mult_left_mono power_mono) auto
+    also have \<open>\<dots> =  2 * real (length xs) * exp (-real thresh / 12)\<close>
+      unfolding exp_of_nat_mult[symmetric] by simp
+    also have \<open>\<dots> \<le> 2 * real (length xs) * exp (-(12 / \<epsilon> ^ 2 * ln (6 * real (length xs) / \<delta>))/12)\<close>
+      using assms(3) by (intro mult_left_mono iffD2[OF exp_le_cancel_iff] divide_right_mono) auto
+    also have \<open>\<dots> = 2 * real (length xs) * exp (-ln (6 * real (length xs) / \<delta>) / \<epsilon>^2 )\<close>
+      by auto
+    also have \<open>\<dots> \<le> 2 * real (length xs) * exp (-ln (6 * real (length xs) / \<delta>) / 1 )\<close>
+      using assms(1,2) False 
+      by (intro mult_left_mono iffD2[OF exp_le_cancel_iff] divide_left_mono_neg power_le_one) 
+        (auto intro!:ln_ge_zero simp:divide_simps)
+    also have \<open>\<dots> = 2 * real (length xs) * exp (ln (inverse (6 * real (length xs) / \<delta>)))\<close>
+      using False assms(2) by (subst ln_inverse[symmetric]) auto
+    also have \<open>\<dots> = 2 * real (length xs) / (6 * real (length xs) / \<delta>)\<close>
+      using assms(1,2) False by (subst exp_ln) auto
+    also have \<open>\<dots> = \<delta> / 3\<close> using False assms(2) by auto
+    also have \<open>\<dots> \<le> \<delta>\<close> using assms(2) by auto
+    finally have \<open>2 * real (length xs) * f^thresh \<le> \<delta>\<close> by simp
+    thus ?thesis unfolding \<alpha>_def by simp
+  qed
+  finally have f:\<open>prob_fail (run_steps xs) \<le> \<delta> / 2\<close> by simp
+
+  have g:\<open>spmf_of_pmf (abs.run_steps xs) = foldM_spmf (\<lambda>x \<sigma>. step_1 x \<sigma> \<bind> step_2) xs initial_state\<close>
+    unfolding abs.run_steps_def foldM_spmf_of_pmf_eq(2)[symmetric] 
+    unfolding spmf_of_pmf_def map_pmf_def c b a
+    by (simp add:bind_assoc_pmf bind_spmf_def bind_return_pmf)
+
+  have \<open>?L \<le> measure (run_steps xs) {None} + 
+    measure (measure_spmf (run_steps xs)) {x. \<bar>estimate x - R\<bar> > \<epsilon> * R}\<close>
+    unfolding measure_measure_spmf_conv_measure_pmf by (intro pmf_add) (auto split:option.split_asm)
+  also have \<open>\<dots> \<le> \<delta> / 2 + measure (measure_spmf (run_steps xs)) {x. \<bar>estimate x - R\<bar> > \<epsilon> * R}\<close>
+    unfolding measure_pmf_single by (intro add_mono f order.refl)
+  also have \<open>\<dots> \<le> \<delta>/2+measure(measure_spmf (spmf_of_pmf (abs.run_steps xs))) {x. \<bar>estimate x-R\<bar>>\<epsilon>*R}\<close>
+    using ord_spmf_eqD_emeasure[OF ord_spmf_run_steps] unfolding measure_spmf.emeasure_eq_measure g
+    by (intro add_mono) auto
+  also have \<open>\<dots> \<le> \<delta> / 2 + measure (abs.run_steps xs) {x. \<bar>estimate x - R\<bar> > \<epsilon> * R}\<close>
+    using measure_spmf_map_pmf_Some spmf_of_pmf_def by auto
+  also have \<open>\<dots> \<le> \<delta> / 2 + \<delta> / 2\<close>
+    using assms(1-3) unfolding R_def by (intro add_mono abs.correctness) auto
+  finally show ?thesis by simp
+qed
+
+end
+
+end
